theories/sim/program.v
@@ -30,7 +30,7 @@ Proof.
   - eapply (sim_body_step_over_call _ _ init_res ε _ (ValR _) [] []); [done|..].
     { intros fid fn_src. specialize (FUNS fid fn_src). naive_solver. }
     intros. simpl. exists 1%nat.
-    apply (sim_body_result _ _ _ _ (ValR vs) (ValR vt)).
+    apply: sim_body_result.
     intros VALID.
     have ?: rrel (init_res ⋅ r') vs vt.
     { eapply rrel_mono; [done|apply cmra_included_r|exact VRET]. }
